\section{COMBINATORICS}
\subsection{Catalan numbers}
\bit
\w Given a sequence of $n$ elements, the number of parenthesizations 
   can be defined as a recurrence:
\[ C(n) = \left\{\begin{array}{ll}
   1 & \mbox{if\ } n = 1,\\
   \sum_{k=1}^{n-1}C(k)C(n-k) & \mbox{if\ } n \ge 2,\\
	    \end{array}\right.\]
   This number is called the \bb{Catalan number} and
  $C(n) = \frac{1}{n+1}{2n \choose n} = {2n \choose n} - {2n \choose 2n-1}
   = \Omega\left(4^n/n^{3/2}\right)$.
\eit

\subsection{Fibonacci sequence}
\bit
\w Let $(F_i)$ be the sequence of Fibonacci numbers.
\w $\phi = (1 + \sqrt{5})/2$ is \bb{golden ratio} and is a solution for 
   the equation $\phi^2 = \phi + 1$.
\w \bb{Theorem}: $\phi^{n-2} \le F_n \le \phi^{n-1}$.
\eit

	

\subsection{First-order linear recurrences}
\bit
\w Let a recurrence of the form
	$a_nT_n = b_nT_{n-1} + c_n$ be given.
\ben
\w Multiply both sides by a {\bf{}summation factor} $s_n$:
	\[ s_na_nT_n = s_nb_nT_{n-1} + s_nc_n\]
	where we set {$s_nb_n = s_{n-1}a_{n-1}$}.
\w Substitute $S_n = s_na_nT_n$, which renders
	\[ S_n = S_{n-1} + s_nc_n, \]
	which is easy to solve.
\w [(*)] {\em The crucial point is how we can choose $s_n$.}
	Since $s_nb_n = s_{n-1}a_{n-1}$ should
	be satisfied,
	\[s_n  =  s_{n-1}\frac{a_{n-1}}{b_n} =
	s_{n-2}\frac{a_{n-2}}{b_{n-1}}\frac{a_{n-1}}{b_n} = \frac{a_{n-1}a_{n-2}\cdots{a_1}}{b_nb_{n-1}\cdots{b_2}}.\]

\een
\eit

\subsection{Perturbation method for computing summations}
\bit
\w 
Let $S_n$ be a unknown sum, $S_n = \sum_{0\le{k}\le n} a_k$,
which we want to evaluate.
\ben
\w {\em Rewrite `$S_{n+1}$' in two ways\/} ({\bf{}name and conquer}),
by splitting off both its last term and and its first term.
\begin{eqnarray*}
S_n + a_{n+1} = \sum_{0\le{k}\le n+1}a_k & = &
	a_0 + \sum_{1\le{k}\le{n+1}}a_k \\
	& = & a_0 + \sum_{1\le{k+1}\le n+1} a_{k+1} \\
	& = & a_0 + \sum_{0\le k\le n} a_{k+1}.
\end{eqnarray*}
\w Now express the last sum in terms of $S_n$.
\w Solve the equation.
\een
\eit
%% \paragraph{Example of perturbation method} Find the sum of 
%% {\em{}geometric progression\/},
%% 	\[ S_n = \sum_{0\le{k}\le n} ax^k.\]
%% \ben
%% \w Rewrite:
%% 	\begin{eqnarray*}
%% 	S_n + ax^{n+1} & = & ax^0 + \sum_{1\le{k}\le n+1}ax^k \\
%% 		& = & a + \sum_{0\le k \le n} ax^{k+1}
%% 	\end{eqnarray*}
%% \w Express:
%% 	\begin{eqnarray*}
%% 	\sum_{0\le k \le n} ax^{k+1} & = & \sum_{0\le k \le n}ax^k x\\
%% 		& = & xS_n
%% 	\end{eqnarray*}
%% \w Solve:
%% 	\begin{eqnarray*}
%% 	S_n + ax^{n+1} & = & a + xS_n \\
%% 	(1-x)S_n & = & a(1 - x^{n+1}) \\
%% 	S_n & = & \frac{a(1-x^{n+1})}{1-x}, \quad x \ne 1.
%% 	\end{eqnarray*}
%% \een

